\documentclass{article}
\usepackage{epsfig}
\usepackage{indentfirst}
\usepackage{amsmath}
\usepackage{amsfonts}
\pagestyle{empty}
\begin{document}
$ \mathbb F_{2^{64}}$
\pagebreak

$ f(x) = x^{64} + x^4 + x^3 + x + 1 \in \mathbb F_2[x]$
\pagebreak

$ \mathbb F_{2^{128}}$
\pagebreak

$ f(x) = x^{128} + x^7 + x^2 + x + 1 \in \mathbb F_2[x]$
\pagebreak

$\Delta \equiv -16(4a^3 + 27b^2) \pmod{p} $
\pagebreak

$ t \pmod{q} $
\pagebreak

$ t \cdot t^{-1} \equiv 1 \pmod{q}$
\pagebreak

$ p $
\pagebreak

$ 2^{n-32} < p < 2^n $
\pagebreak

$ n $
\pagebreak

$ q $
\pagebreak

$ P $
\pagebreak

$ Q $
\pagebreak

$ P = (x:y:z) $
\pagebreak

$ yz^2 \equiv x^3 + axz^2 + bz^3 \pmod{p}$
\pagebreak

$P$
\pagebreak

$ 2P = (x_3:y_3:z_3)$
\pagebreak

$ P = (x_1: y_1: z_1) $
\pagebreak

$ Q = (x_2:y_2:z_2)$
\pagebreak

$ P+Q = (x_3:y_3:z_3)$
\pagebreak

$ P$
\pagebreak

$ P = \left( \frac{x}{z} \pmod{p}, \frac{y}{z} \pmod{p}, 1\right) $
\pagebreak

$ k $
\pagebreak

$ Q = [k]P = \underbrace{P+ \cdots + P}_{k\text{~раз}}$
\pagebreak

$ [q]P = \mathcal O$
\pagebreak

$ \mathcal O $
\pagebreak

$ P=(x:y:z) $
\pagebreak

$ y^2z \equiv x^3 + axz^2 + bz^3 \pmod{p} $
\pagebreak

$ y^2 \equiv x^3 + ax + b \pmod{p} $
\pagebreak

$P=(x_P, y_P)$
\pagebreak

$ m $
\pagebreak

$ m = dq $
\pagebreak

$ d $
\pagebreak

$ n, n_q, r_2$
\pagebreak

$ r = 2^{256}$
\pagebreak

$ r=2^{512}$
\pagebreak

$ n \equiv n_0 \pmod{2^{64}}$
\pagebreak

$ n_0 \equiv -p^{-1} \pmod{r}$
\pagebreak

$ r_2 $
\pagebreak

$ r_2 \equiv r^2 \pmod{p}$
\pagebreak

$ a $
\pagebreak

$ b $
\pagebreak

$ r^2$
\pagebreak

$ n_q $
\pagebreak

$ q$
\pagebreak

$ 2^{256} $
\pagebreak

$ 0 \leq n \leq 32 $
\pagebreak

$\mathbb F_{2^8}$
\pagebreak

$ \mathbb Z_{2^{32}}$
\pagebreak

$ k_1, \ldots, k_n$
\pagebreak

$ x_1, \ldots, x_n$
\pagebreak

$ k_1 + x_1 \pmod{2^{32}}, \ldots, k_n + x_n \pmod{2^{32}}$
\pagebreak

$ y_1, \ldots, y_n$
\pagebreak

$ \mathbb Z_{2^{64}} $
\pagebreak

$ \pi $
\pagebreak

$ \overline x $
\pagebreak

$ f(x,y)\in\mathbb Z[x]$
\pagebreak

$ f(x,y) = \frac{1}{2}\left( (x+y)^2 + x + 3y \right)$
\pagebreak

$ \pi(x,y) = const \oplus \left\{ \begin{array}{ll} f(x,y), & x+y < 2^{32}, \\ \overline{f(\overline{x},\overline{y})}, & 2^{32} \le x+y < 2^{64}. \end{array} \right.$
\pagebreak

$ x \in \mathbb Z_{2^{32}} $
\pagebreak

$ y \in \mathbb Z_{2^{32}} $
\pagebreak

$ \mathbb Z_{2^n} $
\pagebreak

$ z \equiv x + y \pmod{2^n}$
\pagebreak

$ x + y = z + r\cdot 2^n$
\pagebreak

$ z \equiv x - y \pmod{2^n}$
\pagebreak

$ z = x - y + r\cdot 2^n$
\pagebreak

$ x $
\pagebreak

$ x$
\pagebreak

$ z $
\pagebreak

$ x, y \in \mathbb Z_{2^n} $
\pagebreak

$ z \in \mathbb Z_{2^n} $
\pagebreak

$ z = x\cdot y$
\pagebreak

$ r $
\pagebreak

$ r \equiv u \pmod{p}$
\pagebreak

$ u $
\pagebreak

$ u, p \in \mathbb Z_{2^n}$
\pagebreak

$ p > 2^{n-32}$
\pagebreak

$ z \equiv x + y \pmod{p}$
\pagebreak

$ z \equiv 2x \pmod{p}$
\pagebreak

$ x \equiv x_0r \pmod{p} $
\pagebreak

$ y \equiv y_0r \pmod{p} $
\pagebreak

$ z \equiv x_0y_0r \pmod{p}$
\pagebreak

$ rs - np = 1$
\pagebreak

$ xr $
\pagebreak

$z \equiv (x^k)r \pmod{p}$
\pagebreak

$ x^k \pmod{p}$
\pagebreak

$2^{256}$
\pagebreak

$2^{512}$
\pagebreak

$ x_{n+1} \equiv a\cdot x_n + c \pmod{2^{64}}, $
\pagebreak

$ a = 125643267795740073 $
\pagebreak

$ b = 506098983240188723. $
\pagebreak

$ \gamma_n = \displaystyle\frac{x_n - \hat x_n}{2^{24}} \pmod{256}, $
\pagebreak

$\hat x_n \equiv x_n \pmod{2^{24}}. $
\pagebreak

$ \mathbb Z_q$
\pagebreak

$ km^{-1} \pmod{q} $
\pagebreak

$ \zeta $
\pagebreak

$ k \equiv k\zeta \pmod{q} $
\pagebreak

$ m \equiv m\zeta^{-1} \pmod{q} $
\pagebreak

$ e $
\pagebreak

$ C = [k]P$
\pagebreak

$ C $
\pagebreak

$ r \equiv x \pmod{q}$
\pagebreak

$ s $
\pagebreak

$ s \equiv rd + ke \pmod{q}$
\pagebreak

$ r||s $
\pagebreak

$ v $
\pagebreak

$ k \oplus v $
\pagebreak

$ \mathbb V^n $
\pagebreak

$ 2^{512} $
\pagebreak

$ \Sigma $
\pagebreak

$ 2^8 $
\pagebreak

\end{document}
